\begin{solution}
The inverse function of $F$ is equal to $F^{-1}(x,y,z) = (y \cdot \sin(2z) + x \cdot \cos(2z), 2z)$.\\[0.2cm]
Since $F(u,v) = (u \cdot \cos(v), u \cdot \sin(v), 0.5 v)$, if we define $F^{-1}(x,y,z) = (u,v)$ it implies that $v=2z$. To determine the value of $u$ we leverage the fact that $\sin^2(v) + \cos^2(v) = 1$ which implies:
$$\begin{aligned}
	u &= u \cdot (\sin^2(v) + \cos^2(v))\\
	&= (u \cdot \sin(v)) \cdot \sin(v) + (u \cdot \cos(v)) \cdot \cos(v) \\
	&= y \cdot \sin(v) + x \cdot \cos(v) \\
	&= y \cdot \sin(2z) + x \cdot \cos(2z).
\end{aligned} $$
\end{solution}
